@prefix : <https://w3id.org/dlprovenance#> .
@prefix owl: <http://www.w3.org/2002/07/owl#> .
@prefix rdf: <http://www.w3.org/1999/02/22-rdf-syntax-ns#> .
@prefix xml: <http://www.w3.org/XML/1998/namespace> .
@prefix xsd: <http://www.w3.org/2001/XMLSchema#> .
@prefix rdfs: <http://www.w3.org/2000/01/rdf-schema#> .
@base <https://w3id.org/dlprovenance#> .

[ rdf:type owl:Ontology
 ] .

#################################################################
#    Object Properties
#################################################################

###  https://w3id.org/dlprovenance#hasCodeRepository
:hasCodeRepository rdf:type owl:ObjectProperty ;
                   rdfs:domain :DeepLearningModel ;
                   rdfs:range :CodeRepository ;
                   rdfs:comment "A relation between a deep learning model and its code repository." ;
                   rdfs:label "hasCodeRepository" .


###  https://w3id.org/dlprovenance#hasCodeRepositoryLink
:hasCodeRepositoryLink rdf:type owl:ObjectProperty ;
                       rdfs:domain :DeepLearningModel ;
                       rdfs:range :CodeRepositoryLink ;
                       rdfs:comment "A relation between a deep learning model and its code repository link." ;
                       rdfs:label "hasCodeRepositoryLink" .


###  https://w3id.org/dlprovenance#hasDataAnnotationTechnique
:hasDataAnnotationTechnique rdf:type owl:ObjectProperty ;
                            rdfs:domain :DeepLearningModel ;
                            rdfs:range :DataAnnotationTechnique ;
                            rdfs:comment "A relation between a deep learning model and its data annotation technique." ;
                            rdfs:label "hasDataAnnotationTechnique" .


###  https://w3id.org/dlprovenance#hasDataAugmentationTechnique
:hasDataAugmentationTechnique rdf:type owl:ObjectProperty ;
                              rdfs:domain :DeepLearningModel ;
                              rdfs:range :DataAugmentationTechnique ;
                              rdfs:comment "A relation between a deep learning model and its data augmentation technique." ;
                              rdfs:label "hasDataAugmentationTechnique" .


###  https://w3id.org/dlprovenance#hasDataBiasTechnique
:hasDataBiasTechnique rdf:type owl:ObjectProperty ;
                      rdfs:domain :DeepLearningModel ;
                      rdfs:range :DataBiasTechnique ;
                      rdfs:comment "A relation between a deep learning model and its data bias technique." ;
                      rdfs:label "hasDataBiasTechnique" .


###  https://w3id.org/dlprovenance#hasDataFormat
:hasDataFormat rdf:type owl:ObjectProperty ;
               rdfs:domain :DeepLearningModel ;
               rdfs:range :DataFormat ;
               rdfs:comment "A relation between a deep learning model and its data format." ;
               rdfs:label "hasDataFormat" .


###  https://w3id.org/dlprovenance#hasDataRepository
:hasDataRepository rdf:type owl:ObjectProperty ;
                   rdfs:domain :DeepLearningModel ;
                   rdfs:range :DataRepository ;
                   rdfs:comment "A relation between a deep learning model and its data repository." ;
                   rdfs:label "hasDataRepository" .


###  https://w3id.org/dlprovenance#hasDataRepositoryLink
:hasDataRepositoryLink rdf:type owl:ObjectProperty ;
                       rdfs:domain :DeepLearningModel ;
                       rdfs:range :DataRepositoryLink ;
                       rdfs:comment "A relation between a deep learning model and its data repository link." ;
                       rdfs:label "hasDataRepositoryLink" .


###  https://w3id.org/dlprovenance#hasDataSplitCriteria
:hasDataSplitCriteria rdf:type owl:ObjectProperty ;
                      rdfs:domain :DeepLearningModel ;
                      rdfs:range :DataSplitCriteria ;
                      rdfs:comment "A relation between a deep learning model and its data split criteria." ;
                      rdfs:label "hasDataSplitCriteria" .


###  https://w3id.org/dlprovenance#hasDataset
:hasDataset rdf:type owl:ObjectProperty ;
            rdfs:domain :DeepLearningModel ;
            rdfs:range :Dataset ;
            rdfs:comment "A relation between a deep learning model and its dataset." ;
            rdfs:label "hasDataset" .


###  https://w3id.org/dlprovenance#hasDeepLearningModel
:hasDeepLearningModel rdf:type owl:ObjectProperty ;
                      rdfs:domain :DeepLearningModel ;
                      rdfs:range :DeepLearningModel ;
                      rdfs:comment "A relation between a deep learning model and its deep learning model." ;
                      rdfs:label "hasDeepLearningModel" .


###  https://w3id.org/dlprovenance#hasDeploymentPlatform
:hasDeploymentPlatform rdf:type owl:ObjectProperty ;
                       rdfs:domain :DeepLearningModel ;
                       rdfs:range :DeploymentPlatform ;
                       rdfs:comment "A relation between a deep learning model and its deployment platform." ;
                       rdfs:label "hasDeploymentPlatform" .


###  https://w3id.org/dlprovenance#hasFramework
:hasFramework rdf:type owl:ObjectProperty ;
              rdfs:domain :DeepLearningModel ;
              rdfs:range :Framework ;
              rdfs:comment "A relation between a deep learning model and its framework." ;
              rdfs:label "hasFramework" .


###  https://w3id.org/dlprovenance#hasGeneralizabilityMeasure
:hasGeneralizabilityMeasure rdf:type owl:ObjectProperty ;
                            rdfs:domain :DeepLearningModel ;
                            rdfs:range :GeneralizabilityMeasure ;
                            rdfs:comment "A relation between a deep learning model and its generalizability measure." ;
                            rdfs:label "hasGeneralizabilityMeasure" .


###  https://w3id.org/dlprovenance#hasHardwareResource
:hasHardwareResource rdf:type owl:ObjectProperty ;
                     rdfs:domain :DeepLearningModel ;
                     rdfs:range :HardwareResource ;
                     rdfs:comment "A relation between a deep learning model and its hardware resource." ;
                     rdfs:label "hasHardwareResource" .


###  https://w3id.org/dlprovenance#hasHyperparameter
:hasHyperparameter rdf:type owl:ObjectProperty ;
                   rdfs:domain :DeepLearningModel ;
                   rdfs:range :Hyperparameter ;
                   rdfs:comment "A relation between a deep learning model and its hyperparameter." ;
                   rdfs:label "hasHyperparameter" .


###  https://w3id.org/dlprovenance#hasHyperparameterOptimization
:hasHyperparameterOptimization rdf:type owl:ObjectProperty ;
                               rdfs:domain :DeepLearningModel ;
                               rdfs:range :HyperparameterOptimization ;
                               rdfs:comment "A relation between a deep learning model and its hyperparameter optimization." ;
                               rdfs:label "hasHyperparameterOptimization" .


###  https://w3id.org/dlprovenance#hasMethod
:hasMethod rdf:type owl:ObjectProperty ;
           rdfs:domain :DeepLearningModel ;
           rdfs:range :Method ;
           rdfs:comment "A relation between a deep learning model and its method." ;
           rdfs:label "hasMethod" .


###  https://w3id.org/dlprovenance#hasModelDeploymentProcess
:hasModelDeploymentProcess rdf:type owl:ObjectProperty ;
                           rdfs:domain :DeepLearningModel ;
                           rdfs:range :ModelDeploymentProcess ;
                           rdfs:comment "A relation between a deep learning model and its model deployment process." ;
                           rdfs:label "hasModelDeploymentProcess" .


###  https://w3id.org/dlprovenance#hasModelPerformanceMonitoringStrategy
:hasModelPerformanceMonitoringStrategy rdf:type owl:ObjectProperty ;
                                       rdfs:domain :DeepLearningModel ;
                                       rdfs:range :ModelPerformanceMonitoringStrategy ;
                                       rdfs:comment "A relation between a deep learning model and its model performance monitoring strategy." ;
                                       rdfs:label "hasModelPerformanceMonitoringStrategy" .


###  https://w3id.org/dlprovenance#hasModelPurpose
:hasModelPurpose rdf:type owl:ObjectProperty ;
                 rdfs:domain :DeepLearningModel ;
                 rdfs:range :ModelPurpose ;
                 rdfs:comment "A relation between a deep learning model and its model purpose." ;
                 rdfs:label "hasModelPurpose" .


###  https://w3id.org/dlprovenance#hasOptimizationTechnique
:hasOptimizationTechnique rdf:type owl:ObjectProperty ;
                          rdfs:domain :DeepLearningModel ;
                          rdfs:range :OptimizationTechnique ;
                          rdfs:comment "A relation between a deep learning model and its optimization technique." ;
                          rdfs:label "hasOptimizationTechnique" .


###  https://w3id.org/dlprovenance#hasPerformanceMetric
:hasPerformanceMetric rdf:type owl:ObjectProperty ;
                      rdfs:domain :DeepLearningModel ;
                      rdfs:range :PerformanceMetric ;
                      rdfs:comment "A relation between a deep learning model and its performance metric." ;
                      rdfs:label "hasPerformanceMetric" .


###  https://w3id.org/dlprovenance#hasPostprocessingStep
:hasPostprocessingStep rdf:type owl:ObjectProperty ;
                       rdfs:domain :DeepLearningModel ;
                       rdfs:range :PostprocessingStep ;
                       rdfs:comment "A relation between a deep learning model and its postprocessing step." ;
                       rdfs:label "hasPostprocessingStep" .


###  https://w3id.org/dlprovenance#hasPreprocessingStep
:hasPreprocessingStep rdf:type owl:ObjectProperty ;
                      rdfs:domain :DeepLearningModel ;
                      rdfs:range :PreprocessingStep ;
                      rdfs:comment "A relation between a deep learning model and its preprocessing step." ;
                      rdfs:label "hasPreprocessingStep" .


###  https://w3id.org/dlprovenance#hasRandomnessStrategy
:hasRandomnessStrategy rdf:type owl:ObjectProperty ;
                       rdfs:domain :DeepLearningModel ;
                       rdfs:range :RandomnessStrategy ;
                       rdfs:comment "A relation between a deep learning model and its randomness strategy." ;
                       rdfs:label "hasRandomnessStrategy" .


###  https://w3id.org/dlprovenance#hasRawData
:hasRawData rdf:type owl:ObjectProperty ;
            rdfs:domain :DeepLearningModel ;
            rdfs:range :RawData ;
            rdfs:comment "A relation between a deep learning model and its raw data." ;
            rdfs:label "hasRawData" .


###  https://w3id.org/dlprovenance#hasRegularizationMethod
:hasRegularizationMethod rdf:type owl:ObjectProperty ;
                         rdfs:domain :DeepLearningModel ;
                         rdfs:range :RegularizationMethod ;
                         rdfs:comment "A relation between a deep learning model and its regularization method." ;
                         rdfs:label "hasRegularizationMethod" .


###  https://w3id.org/dlprovenance#hasTrainingCompletionCriteria
:hasTrainingCompletionCriteria rdf:type owl:ObjectProperty ;
                               rdfs:domain :DeepLearningModel ;
                               rdfs:range :TrainingCompletionCriteria ;
                               rdfs:comment "A relation between a deep learning model and its training completion criteria." ;
                               rdfs:label "hasTrainingCompletionCriteria" .


###  https://w3id.org/dlprovenance#isCodeRepositoryLinkOf
:isCodeRepositoryLinkOf rdf:type owl:ObjectProperty ;
                        rdfs:domain :CodeRepositoryLink ;
                        rdfs:range :DeepLearningModel ;
                        rdfs:comment "A relation between a code repository link and its deep learning model." ;
                        rdfs:label "isCodeRepositoryLinkOf" .


###  https://w3id.org/dlprovenance#isCodeRepositoryOf
:isCodeRepositoryOf rdf:type owl:ObjectProperty ;
                    rdfs:domain :CodeRepository ;
                    rdfs:range :DeepLearningModel ;
                    rdfs:comment "A relation between a code repository and its deep learning model." ;
                    rdfs:label "isCodeRepositoryOf" .


###  https://w3id.org/dlprovenance#isDataAnnotationTechniqueOf
:isDataAnnotationTechniqueOf rdf:type owl:ObjectProperty ;
                             rdfs:domain :DataAnnotationTechnique ;
                             rdfs:range :DeepLearningModel ;
                             rdfs:comment "A relation between a data annotation technique and its deep learning model." ;
                             rdfs:label "isDataAnnotationTechniqueOf" .


###  https://w3id.org/dlprovenance#isDataAugmentationTechniqueOf
:isDataAugmentationTechniqueOf rdf:type owl:ObjectProperty ;
                               rdfs:domain :DataAugmentationTechnique ;
                               rdfs:range :DeepLearningModel ;
                               rdfs:comment "A relation between a data augmentation technique and its deep learning model." ;
                               rdfs:label "isDataAugmentationTechniqueOf" .


###  https://w3id.org/dlprovenance#isDataBiasTechniqueOf
:isDataBiasTechniqueOf rdf:type owl:ObjectProperty ;
                       rdfs:domain :DataBiasTechnique ;
                       rdfs:range :DeepLearningModel ;
                       rdfs:comment "A relation between a data bias technique and its deep learning model." ;
                       rdfs:label "isDataBiasTechniqueOf" .


###  https://w3id.org/dlprovenance#isDataFormatOf
:isDataFormatOf rdf:type owl:ObjectProperty ;
                rdfs:domain :DataFormat ;
                rdfs:range :DeepLearningModel ;
                rdfs:comment "A relation between a data format and its deep learning model." ;
                rdfs:label "isDataFormatOf" .


###  https://w3id.org/dlprovenance#isDataRepositoryLinkOf
:isDataRepositoryLinkOf rdf:type owl:ObjectProperty ;
                        rdfs:domain :DataRepositoryLink ;
                        rdfs:range :DeepLearningModel ;
                        rdfs:comment "A relation between a data repository link and its deep learning model." ;
                        rdfs:label "isDataRepositoryLinkOf" .


###  https://w3id.org/dlprovenance#isDataRepositoryOf
:isDataRepositoryOf rdf:type owl:ObjectProperty ;
                    rdfs:domain :DataRepository ;
                    rdfs:range :DeepLearningModel ;
                    rdfs:comment "A relation between a data repository and its deep learning model." ;
                    rdfs:label "isDataRepositoryOf" .


###  https://w3id.org/dlprovenance#isDataSplitCriteriaOf
:isDataSplitCriteriaOf rdf:type owl:ObjectProperty ;
                       rdfs:domain :DataSplitCriteria ;
                       rdfs:range :DeepLearningModel ;
                       rdfs:comment "A relation between data split criteria and its deep learning model." ;
                       rdfs:label "isDataSplitCriteriaOf" .


###  https://w3id.org/dlprovenance#isDatasetOf
:isDatasetOf rdf:type owl:ObjectProperty ;
             rdfs:domain :Dataset ;
             rdfs:range :DeepLearningModel ;
             rdfs:comment "A relation between a dataset and its deep learning model." ;
             rdfs:label "isDatasetOf" .


###  https://w3id.org/dlprovenance#isDeepLearningModelOf
:isDeepLearningModelOf rdf:type owl:ObjectProperty ;
                       rdfs:domain :DeepLearningModel ;
                       rdfs:range :DeepLearningModel ;
                       rdfs:comment "A relation between a deep learning model and its deep learning model." ;
                       rdfs:label "isDeepLearningModelOf" .


###  https://w3id.org/dlprovenance#isDeploymentPlatformOf
:isDeploymentPlatformOf rdf:type owl:ObjectProperty ;
                        rdfs:domain :DeploymentPlatform ;
                        rdfs:range :DeepLearningModel ;
                        rdfs:comment "A relation between a deployment platform and its deep learning model." ;
                        rdfs:label "isDeploymentPlatformOf" .


###  https://w3id.org/dlprovenance#isFrameworkOf
:isFrameworkOf rdf:type owl:ObjectProperty ;
               rdfs:domain :Framework ;
               rdfs:range :DeepLearningModel ;
               rdfs:comment "A relation between a framework and its deep learning model." ;
               rdfs:label "isFrameworkOf" .


###  https://w3id.org/dlprovenance#isGeneralizabilityMeasureOf
:isGeneralizabilityMeasureOf rdf:type owl:ObjectProperty ;
                             rdfs:domain :GeneralizabilityMeasure ;
                             rdfs:range :DeepLearningModel ;
                             rdfs:comment "A relation between a generalizability measure and its deep learning model." ;
                             rdfs:label "isGeneralizabilityMeasureOf" .


###  https://w3id.org/dlprovenance#isHardwareResourceOf
:isHardwareResourceOf rdf:type owl:ObjectProperty ;
                      rdfs:domain :HardwareResource ;
                      rdfs:range :DeepLearningModel ;
                      rdfs:comment "A relation between a hardware resource and its deep learning model." ;
                      rdfs:label "isHardwareResourceOf" .


###  https://w3id.org/dlprovenance#isHyperparameterOf
:isHyperparameterOf rdf:type owl:ObjectProperty ;
                    rdfs:domain :Hyperparameter ;
                    rdfs:range :DeepLearningModel ;
                    rdfs:comment "A relation between a hyperparameter and its deep learning model." ;
                    rdfs:label "isHyperparameterOf" .


###  https://w3id.org/dlprovenance#isHyperparameterOptimizationOf
:isHyperparameterOptimizationOf rdf:type owl:ObjectProperty ;
                                rdfs:domain :HyperparameterOptimization ;
                                rdfs:range :DeepLearningModel ;
                                rdfs:comment "A relation between a hyperparameter optimization and its deep learning model." ;
                                rdfs:label "isHyperparameterOptimizationOf" .


###  https://w3id.org/dlprovenance#isMethodOf
:isMethodOf rdf:type owl:ObjectProperty ;
            rdfs:domain :Method ;
            rdfs:range :DeepLearningModel ;
            rdfs:comment "A relation between a method and its deep learning model." ;
            rdfs:label "isMethodOf" .


###  https://w3id.org/dlprovenance#isModelDeploymentProcessOf
:isModelDeploymentProcessOf rdf:type owl:ObjectProperty ;
                            rdfs:domain :ModelDeploymentProcess ;
                            rdfs:range :DeepLearningModel ;
                            rdfs:comment "A relation between a model deployment process and its deep learning model." ;
                            rdfs:label "isModelDeploymentProcessOf" .


###  https://w3id.org/dlprovenance#isModelPerformanceMonitoringStrategyOf
:isModelPerformanceMonitoringStrategyOf rdf:type owl:ObjectProperty ;
                                        rdfs:domain :ModelPerformanceMonitoringStrategy ;
                                        rdfs:range :DeepLearningModel ;
                                        rdfs:comment "A relation between a model performance monitoring strategy and its deep learning model." ;
                                        rdfs:label "isModelPerformanceMonitoringStrategyOf" .


###  https://w3id.org/dlprovenance#isModelPurposeOf
:isModelPurposeOf rdf:type owl:ObjectProperty ;
                  rdfs:domain :ModelPurpose ;
                  rdfs:range :DeepLearningModel ;
                  rdfs:comment "A relation between a model purpose and its deep learning model." ;
                  rdfs:label "isModelPurposeOf" .


###  https://w3id.org/dlprovenance#isOptimizationTechniqueOf
:isOptimizationTechniqueOf rdf:type owl:ObjectProperty ;
                           rdfs:domain :OptimizationTechnique ;
                           rdfs:range :DeepLearningModel ;
                           rdfs:comment "A relation between an optimization technique and its deep learning model." ;
                           rdfs:label "isOptimizationTechniqueOf" .


###  https://w3id.org/dlprovenance#isPerformanceMetricOf
:isPerformanceMetricOf rdf:type owl:ObjectProperty ;
                       rdfs:domain :PerformanceMetric ;
                       rdfs:range :DeepLearningModel ;
                       rdfs:comment "A relation between a performance metric and its deep learning model." ;
                       rdfs:label "isPerformanceMetricOf" .


###  https://w3id.org/dlprovenance#isPostprocessingStepOf
:isPostprocessingStepOf rdf:type owl:ObjectProperty ;
                        rdfs:domain :PostprocessingStep ;
                        rdfs:range :DeepLearningModel ;
                        rdfs:comment "A relation between a postprocessing step and its deep learning model." ;
                        rdfs:label "isPostprocessingStepOf" .


###  https://w3id.org/dlprovenance#isPreprocessingStepOf
:isPreprocessingStepOf rdf:type owl:ObjectProperty ;
                       rdfs:domain :PreprocessingStep ;
                       rdfs:range :DeepLearningModel ;
                       rdfs:comment "A relation between a preprocessing step and its deep learning model." ;
                       rdfs:label "isPreprocessingStepOf" .


###  https://w3id.org/dlprovenance#isRandomnessStrategyOf
:isRandomnessStrategyOf rdf:type owl:ObjectProperty ;
                        rdfs:domain :RandomnessStrategy ;
                        rdfs:range :DeepLearningModel ;
                        rdfs:comment "A relation between a randomness strategy and its deep learning model." ;
                        rdfs:label "isRandomnessStrategyOf" .


###  https://w3id.org/dlprovenance#isRawDataOf
:isRawDataOf rdf:type owl:ObjectProperty ;
             rdfs:domain :RawData ;
             rdfs:range :DeepLearningModel ;
             rdfs:comment "A relation between raw data and its deep learning model." ;
             rdfs:label "isRawDataOf" .


###  https://w3id.org/dlprovenance#isRegularizationMethodOf
:isRegularizationMethodOf rdf:type owl:ObjectProperty ;
                          rdfs:domain :RegularizationMethod ;
                          rdfs:range :DeepLearningModel ;
                          rdfs:comment "A relation between a regularization method and its deep learning model." ;
                          rdfs:label "isRegularizationMethodOf" .


###  https://w3id.org/dlprovenance#isTrainingCompletionCriteriaOf
:isTrainingCompletionCriteriaOf rdf:type owl:ObjectProperty ;
                                rdfs:domain :TrainingCompletionCriteria ;
                                rdfs:range :DeepLearningModel ;
                                rdfs:comment "A relation between training completion criteria and its deep learning model." ;
                                rdfs:label "isTrainingCompletionCriteriaOf" .


#################################################################
#    Data properties
#################################################################

###  https://w3id.org/dlprovenance#codeRepositoryLink
:codeRepositoryLink rdf:type owl:DatatypeProperty ;
                    rdfs:domain :CodeRepositoryLink ;
                    rdfs:range xsd:string ;
                    rdfs:comment "The link to the code repository." ;
                    rdfs:label "codeRepositoryLink" .


###  https://w3id.org/dlprovenance#codeRepositoryName
:codeRepositoryName rdf:type owl:DatatypeProperty ;
                    rdfs:domain :CodeRepository ;
                    rdfs:range xsd:string ;
                    rdfs:comment "The name of the code repository." ;
                    rdfs:label "codeRepositoryName" .


###  https://w3id.org/dlprovenance#dataAnnotationTechniqueName
:dataAnnotationTechniqueName rdf:type owl:DatatypeProperty ;
                             rdfs:domain :DataAnnotationTechnique ;
                             rdfs:range xsd:string ;
                             rdfs:comment "The name of the data annotation technique." ;
                             rdfs:label "dataAnnotationTechniqueName" .


###  https://w3id.org/dlprovenance#dataAugmentationTechniqueName
:dataAugmentationTechniqueName rdf:type owl:DatatypeProperty ;
                               rdfs:domain :DataAugmentationTechnique ;
                               rdfs:range xsd:string ;
                               rdfs:comment "The name of the data augmentation technique." ;
                               rdfs:label "dataAugmentationTechniqueName" .


###  https://w3id.org/dlprovenance#dataBiasTechniqueName
:dataBiasTechniqueName rdf:type owl:DatatypeProperty ;
                       rdfs:domain :DataBiasTechnique ;
                       rdfs:range xsd:string ;
                       rdfs:comment "The name of the data bias technique." ;
                       rdfs:label "dataBiasTechniqueName" .


###  https://w3id.org/dlprovenance#dataFormat
:dataFormat rdf:type owl:DatatypeProperty ;
            rdfs:domain :DataFormat ;
            rdfs:range xsd:string ;
            rdfs:comment "The format of the data." ;
            rdfs:label "dataFormat" .


###  https://w3id.org/dlprovenance#dataRepositoryLink
:dataRepositoryLink rdf:type owl:DatatypeProperty ;
                    rdfs:domain :DataRepositoryLink ;
                    rdfs:range xsd:string ;
                    rdfs:comment "The link to the data repository." ;
                    rdfs:label "dataRepositoryLink" .


###  https://w3id.org/dlprovenance#dataRepositoryName
:dataRepositoryName rdf:type owl:DatatypeProperty ;
                    rdfs:domain :DataRepository ;
                    rdfs:range xsd:string ;
                    rdfs:comment "The name of the data repository." ;
                    rdfs:label "dataRepositoryName" .


###  https://w3id.org/dlprovenance#dataSplitCriteriaName
:dataSplitCriteriaName rdf:type owl:DatatypeProperty ;
                       rdfs:domain :DataSplitCriteria ;
                       rdfs:range xsd:string ;
                       rdfs:comment "The name of the data split criteria." ;
                       rdfs:label "dataSplitCriteriaName" .


###  https://w3id.org/dlprovenance#datasetName
:datasetName rdf:type owl:DatatypeProperty ;
             rdfs:domain :Dataset ;
             rdfs:range xsd:string ;
             rdfs:comment "The name of the dataset." ;
             rdfs:label "datasetName" .


###  https://w3id.org/dlprovenance#deepLearningModelName
:deepLearningModelName rdf:type owl:DatatypeProperty ;
                       rdfs:domain :DeepLearningModel ;
                       rdfs:range xsd:string ;
                       rdfs:comment "The name of the deep learning model." ;
                       rdfs:label "deepLearningModelName" .


###  https://w3id.org/dlprovenance#deploymentPlatformName
:deploymentPlatformName rdf:type owl:DatatypeProperty ;
                        rdfs:domain :DeploymentPlatform ;
                        rdfs:range xsd:string ;
                        rdfs:comment "The name of the deployment platform." ;
                        rdfs:label "deploymentPlatformName" .


###  https://w3id.org/dlprovenance#frameworkName
:frameworkName rdf:type owl:DatatypeProperty ;
               rdfs:domain :Framework ;
               rdfs:range xsd:string ;
               rdfs:comment "The name of the framework." ;
               rdfs:label "frameworkName" .


###  https://w3id.org/dlprovenance#generalizabilityMeasureName
:generalizabilityMeasureName rdf:type owl:DatatypeProperty ;
                             rdfs:domain :GeneralizabilityMeasure ;
                             rdfs:range xsd:string ;
                             rdfs:comment "The name of the generalizability measure." ;
                             rdfs:label "generalizabilityMeasureName" .


###  https://w3id.org/dlprovenance#hardwareResourceName
:hardwareResourceName rdf:type owl:DatatypeProperty ;
                      rdfs:domain :HardwareResource ;
                      rdfs:range xsd:string ;
                      rdfs:comment "The name of the hardware resource." ;
                      rdfs:label "hardwareResourceName" .


###  https://w3id.org/dlprovenance#hyperparameterName
:hyperparameterName rdf:type owl:DatatypeProperty ;
                    rdfs:domain :Hyperparameter ;
                    rdfs:range xsd:string ;
                    rdfs:comment "The name of the hyperparameter." ;
                    rdfs:label "hyperparameterName" .


###  https://w3id.org/dlprovenance#hyperparameterOptimizationName
:hyperparameterOptimizationName rdf:type owl:DatatypeProperty ;
                                rdfs:domain :HyperparameterOptimization ;
                                rdfs:range xsd:string ;
                                rdfs:comment "The name of the hyperparameter optimization." ;
                                rdfs:label "hyperparameterOptimizationName" .


###  https://w3id.org/dlprovenance#methodName
:methodName rdf:type owl:DatatypeProperty ;
            rdfs:domain :Method ;
            rdfs:range xsd:string ;
            rdfs:comment "The name of the method." ;
            rdfs:label "methodName" .


###  https://w3id.org/dlprovenance#modelDeploymentProcessName
:modelDeploymentProcessName rdf:type owl:DatatypeProperty ;
                            rdfs:domain :ModelDeploymentProcess ;
                            rdfs:range xsd:string ;
                            rdfs:comment "The name of the model deployment process." ;
                            rdfs:label "modelDeploymentProcessName" .


###  https://w3id.org/dlprovenance#modelPerformanceMonitoringStrategyName
:modelPerformanceMonitoringStrategyName rdf:type owl:DatatypeProperty ;
                                        rdfs:domain :ModelPerformanceMonitoringStrategy ;
                                        rdfs:range xsd:string ;
                                        rdfs:comment "The name of the model performance monitoring strategy." ;
                                        rdfs:label "modelPerformanceMonitoringStrategyName" .


###  https://w3id.org/dlprovenance#modelPurposeName
:modelPurposeName rdf:type owl:DatatypeProperty ;
                  rdfs:domain :ModelPurpose ;
                  rdfs:range xsd:string ;
                  rdfs:comment "The name of the model purpose." ;
                  rdfs:label "modelPurposeName" .


###  https://w3id.org/dlprovenance#optimizationTechniqueName
:optimizationTechniqueName rdf:type owl:DatatypeProperty ;
                           rdfs:domain :OptimizationTechnique ;
                           rdfs:range xsd:string ;
                           rdfs:comment "The name of the optimization technique." ;
                           rdfs:label "optimizationTechniqueName" .


###  https://w3id.org/dlprovenance#performanceMetricName
:performanceMetricName rdf:type owl:DatatypeProperty ;
                       rdfs:domain :PerformanceMetric ;
                       rdfs:range xsd:string ;
                       rdfs:comment "The name of the performance metric." ;
                       rdfs:label "performanceMetricName" .


###  https://w3id.org/dlprovenance#postprocessingStepName
:postprocessingStepName rdf:type owl:DatatypeProperty ;
                        rdfs:domain :PostprocessingStep ;
                        rdfs:range xsd:string ;
                        rdfs:comment "The name of the postprocessing step." ;
                        rdfs:label "postprocessingStepName" .


###  https://w3id.org/dlprovenance#preprocessingStepName
:preprocessingStepName rdf:type owl:DatatypeProperty ;
                       rdfs:domain :PreprocessingStep ;
                       rdfs:range xsd:string ;
                       rdfs:comment "The name of the preprocessing step." ;
                       rdfs:label "preprocessingStepName" .


###  https://w3id.org/dlprovenance#randomnessStrategyName
:randomnessStrategyName rdf:type owl:DatatypeProperty ;
                        rdfs:domain :RandomnessStrategy ;
                        rdfs:range xsd:string ;
                        rdfs:comment "The name of the randomness strategy." ;
                        rdfs:label "randomnessStrategyName" .


###  https://w3id.org/dlprovenance#regularizationMethodName
:regularizationMethodName rdf:type owl:DatatypeProperty ;
                          rdfs:domain :RegularizationMethod ;
                          rdfs:range xsd:string ;
                          rdfs:comment "The name of the regularization method." ;
                          rdfs:label "regularizationMethodName" .


###  https://w3id.org/dlprovenance#trainingCompletionCriteriaName
:trainingCompletionCriteriaName rdf:type owl:DatatypeProperty ;
                                rdfs:domain :TrainingCompletionCriteria ;
                                rdfs:range xsd:string ;
                                rdfs:comment "The name of the training completion criteria." ;
                                rdfs:label "trainingCompletionCriteriaName" .


#################################################################
#    Classes
#################################################################

###  http://www.w3.org/ns/prov#Entity
<http://www.w3.org/ns/prov#Entity> rdf:type owl:Class .


###  https://w3id.org/dlprovenance#CodeRepository
:CodeRepository rdf:type owl:Class ;
                rdfs:subClassOf <http://www.w3.org/ns/prov#Entity> ;
                rdfs:comment "CodeRepository is a storage location for code."@en ;
                rdfs:label "CodeRepository"@en .


###  https://w3id.org/dlprovenance#CodeRepositoryLink
:CodeRepositoryLink rdf:type owl:Class ;
                    rdfs:subClassOf <http://www.w3.org/ns/prov#Entity> ;
                    rdfs:comment "CodeRepositoryLink is a link to a code repository."@en ;
                    rdfs:label "CodeRepositoryLink"@en .


###  https://w3id.org/dlprovenance#DataAnnotationTechnique
:DataAnnotationTechnique rdf:type owl:Class ;
                         rdfs:subClassOf <http://www.w3.org/ns/prov#Entity> ;
                         rdfs:comment "DataAnnotationTechnique is a method used to add metadata to raw data."@en ;
                         rdfs:label "DataAnnotationTechnique"@en .


###  https://w3id.org/dlprovenance#DataAugmentationTechnique
:DataAugmentationTechnique rdf:type owl:Class ;
                           rdfs:subClassOf <http://www.w3.org/ns/prov#Entity> ;
                           rdfs:comment "DataAugmentationTechnique is a method used to increase the amount of training data."@en ;
                           rdfs:label "DataAugmentationTechnique"@en .


###  https://w3id.org/dlprovenance#DataBiasTechnique
:DataBiasTechnique rdf:type owl:Class ;
                   rdfs:subClassOf <http://www.w3.org/ns/prov#Entity> ;
                   rdfs:comment "DataBiasTechnique is a technique used to introduce bias into data."@en ;
                   rdfs:label "DataBiasTechnique"@en .


###  https://w3id.org/dlprovenance#DataFormat
:DataFormat rdf:type owl:Class ;
            rdfs:subClassOf <http://www.w3.org/ns/prov#Entity> ;
            rdfs:comment "DataFormat is the structure or organization of data."@en ;
            rdfs:label "DataFormat"@en .


###  https://w3id.org/dlprovenance#DataRepository
:DataRepository rdf:type owl:Class ;
                rdfs:subClassOf <http://www.w3.org/ns/prov#Entity> ;
                rdfs:comment "DataRepository is a storage location for data."@en ;
                rdfs:label "DataRepository"@en .


###  https://w3id.org/dlprovenance#DataRepositoryLink
:DataRepositoryLink rdf:type owl:Class ;
                    rdfs:subClassOf <http://www.w3.org/ns/prov#Entity> ;
                    rdfs:comment "DataRepositoryLink is a link to a data repository."@en ;
                    rdfs:label "DataRepositoryLink"@en .


###  https://w3id.org/dlprovenance#DataSplitCriteria
:DataSplitCriteria rdf:type owl:Class ;
                   rdfs:subClassOf <http://www.w3.org/ns/prov#Entity> ;
                   rdfs:comment "DataSplitCriteria is a method used to split the dataset into training and testing datasets."@en ;
                   rdfs:label "DataSplitCriteria"@en .


###  https://w3id.org/dlprovenance#Dataset
:Dataset rdf:type owl:Class ;
         rdfs:subClassOf <http://www.w3.org/ns/prov#Entity> ;
         rdfs:comment "Dataset is a collection of data."@en ;
         rdfs:label "Dataset"@en .


###  https://w3id.org/dlprovenance#DeepLearningModel
:DeepLearningModel rdf:type owl:Class ;
                   rdfs:subClassOf <http://www.w3.org/ns/prov#Entity> ;
                   rdfs:comment "DeepLearningModel is a machine learning model that uses deep learning."@en ;
                   rdfs:label "DeepLearningModel"@en .


###  https://w3id.org/dlprovenance#DeploymentPlatform
:DeploymentPlatform rdf:type owl:Class ;
                    rdfs:subClassOf <http://www.w3.org/ns/prov#Entity> ;
                    rdfs:comment "DeploymentPlatform is a platform used to deploy a machine learning model."@en ;
                    rdfs:label "DeploymentPlatform"@en .


###  https://w3id.org/dlprovenance#Framework
:Framework rdf:type owl:Class ;
           rdfs:subClassOf <http://www.w3.org/ns/prov#Entity> ;
           rdfs:comment "Framework is a software framework used to develop machine learning models."@en ;
           rdfs:label "Framework"@en .


###  https://w3id.org/dlprovenance#GeneralizabilityMeasure
:GeneralizabilityMeasure rdf:type owl:Class ;
                         rdfs:subClassOf <http://www.w3.org/ns/prov#Entity> ;
                         rdfs:comment "GeneralizabilityMeasure is a measure used to evaluate the generalizability of a machine learning model."@en ;
                         rdfs:label "GeneralizabilityMeasure"@en .


###  https://w3id.org/dlprovenance#HardwareResource
:HardwareResource rdf:type owl:Class ;
                  rdfs:subClassOf <http://www.w3.org/ns/prov#Entity> ;
                  rdfs:comment "HardwareResource is a hardware resource used to train a machine learning model."@en ;
                  rdfs:label "HardwareResource"@en .


###  https://w3id.org/dlprovenance#Hyperparameter
:Hyperparameter rdf:type owl:Class ;
                rdfs:subClassOf <http://www.w3.org/ns/prov#Entity> ;
                rdfs:comment "Hyperparameter is a parameter whose value is set before the learning process begins."@en ;
                rdfs:label "Hyperparameter"@en .


###  https://w3id.org/dlprovenance#HyperparameterOptimization
:HyperparameterOptimization rdf:type owl:Class ;
                            rdfs:subClassOf <http://www.w3.org/ns/prov#Entity> ;
                            rdfs:comment "HyperparameterOptimization is the process of finding the best hyperparameters for a machine learning model."@en ;
                            rdfs:label "HyperparameterOptimization"@en .


###  https://w3id.org/dlprovenance#Method
:Method rdf:type owl:Class ;
        rdfs:subClassOf <http://www.w3.org/ns/prov#Entity> ;
        rdfs:comment "Method is a specific procedure or set of procedures used to perform a particular task."@en ;
        rdfs:label "Method"@en .


###  https://w3id.org/dlprovenance#ModelDeploymentProcess
:ModelDeploymentProcess rdf:type owl:Class ;
                        rdfs:subClassOf <http://www.w3.org/ns/prov#Entity> ;
                        rdfs:comment "ModelDeploymentProcess is a process used to deploy a machine learning model."@en ;
                        rdfs:label "ModelDeploymentProcess"@en .


###  https://w3id.org/dlprovenance#ModelPerformanceMonitoringStrategy
:ModelPerformanceMonitoringStrategy rdf:type owl:Class ;
                                    rdfs:subClassOf <http://www.w3.org/ns/prov#Entity> ;
                                    rdfs:comment "ModelPerformanceMonitoringStrategy is a strategy used to monitor the performance of a machine learning model."@en ;
                                    rdfs:label "ModelPerformanceMonitoringStrategy"@en .


###  https://w3id.org/dlprovenance#ModelPurpose
:ModelPurpose rdf:type owl:Class ;
              rdfs:subClassOf <http://www.w3.org/ns/prov#Entity> ;
              rdfs:comment "ModelPurpose is the purpose of a machine learning model."@en ;
              rdfs:label "ModelPurpose"@en .


###  https://w3id.org/dlprovenance#OptimizationTechnique
:OptimizationTechnique rdf:type owl:Class ;
                       rdfs:subClassOf <http://www.w3.org/ns/prov#Entity> ;
                       rdfs:comment "OptimizationTechnique is a method used to optimize a machine learning model."@en ;
                       rdfs:label "OptimizationTechnique"@en .


###  https://w3id.org/dlprovenance#PerformanceMetric
:PerformanceMetric rdf:type owl:Class ;
                   rdfs:subClassOf <http://www.w3.org/ns/prov#Entity> ;
                   rdfs:comment "PerformanceMetric is a metric used to evaluate the performance of a machine learning model."@en ;
                   rdfs:label "PerformanceMetric"@en .


###  https://w3id.org/dlprovenance#PostprocessingStep
:PostprocessingStep rdf:type owl:Class ;
                    rdfs:subClassOf <http://www.w3.org/ns/prov#Entity> ;
                    rdfs:comment "PostprocessingStep is a step used to process the output of a machine learning model."@en ;
                    rdfs:label "PostprocessingStep"@en .


###  https://w3id.org/dlprovenance#PreprocessingStep
:PreprocessingStep rdf:type owl:Class ;
                   rdfs:subClassOf <http://www.w3.org/ns/prov#Entity> ;
                   rdfs:comment "PreprocessingStep is a step used to convert raw data into an understandable format."@en ;
                   rdfs:label "PreprocessingStep"@en .


###  https://w3id.org/dlprovenance#RandomnessStrategy
:RandomnessStrategy rdf:type owl:Class ;
                    rdfs:subClassOf <http://www.w3.org/ns/prov#Entity> ;
                    rdfs:comment "RandomnessStrategy is a strategy used to introduce randomness into a machine learning model."@en ;
                    rdfs:label "RandomnessStrategy"@en .


###  https://w3id.org/dlprovenance#RawData
:RawData rdf:type owl:Class ;
         rdfs:subClassOf <http://www.w3.org/ns/prov#Entity> ;
         rdfs:comment "RawData is the unprocessed data collected from various sources."@en ;
         rdfs:label "RawData"@en .


###  https://w3id.org/dlprovenance#RegularizationMethod
:RegularizationMethod rdf:type owl:Class ;
                      rdfs:subClassOf <http://www.w3.org/ns/prov#Entity> ;
                      rdfs:comment "RegularizationMethod is a method used to prevent overfitting in a machine learning model."@en ;
                      rdfs:label "RegularizationMethod"@en .


###  https://w3id.org/dlprovenance#TrainingCompletionCriteria
:TrainingCompletionCriteria rdf:type owl:Class ;
                            rdfs:subClassOf <http://www.w3.org/ns/prov#Entity> ;
                            rdfs:comment "TrainingCompletionCriteria is a condition that must be met for the training process to be considered complete."@en ;
                            rdfs:label "TrainingCompletionCriteria"@en .


###  Generated by the OWL API (version 4.5.29.2024-05-13T12:11:03Z) https://github.com/owlcs/owlapi
